order-book/verify/Properties/Order/MinimalSingle/DoubleSatisfaction.lean
@@ -1,0 +1,20 @@
+import PlutusCore.UPLC
+import CardanoLedgerApi.V3
+import Blaster
+import Properties.Order.Minimal.DoubleSatisfaction
+import Properties.Order.MinimalSingle.Validator
+
+/-! The single-input restriction prevents double-satisfaction. -/
+
+namespace Properties.Order.MinimalSingle.DoubleSatisfaction
+
+open Properties.Order.Minimal.DoubleSatisfaction (noDoubleSatisfaction)
+open Properties.Order.MinimalSingle.Validator (orderMinimalSingleAcceptsProp)
+
+set_option warn.sorry false
+
+theorem no_double_satisfaction :
+    noDoubleSatisfaction orderMinimalSingleAcceptsProp
+    := by blaster
+
+end Properties.Order.MinimalSingle.DoubleSatisfaction
